src/ecFol.ml
@@ -169,21 +169,21 @@ let f_sampled_from env f1 f2 = f_app (fop_sampled_from (proj_distr_ty env f1.f_t
 let f_secret = f_op CI.CI_Leakable.p_secret [] tconfidentiality
 let f_leaked = f_op CI.CI_Leakable.p_leaked [] tconfidentiality
 
-let fop_undeclassify_invariant_fmap ty1 ty2 =
-  f_op CI.CI_Leakable.p_undeclassify_invariant_fmap [ty1; ty2] (toarrow [
+let fop_secrndasgn_invariant_fmap ty1 ty2 =
+  f_op CI.CI_Leakable.p_secrndasgn_invariant_fmap [ty1; ty2] (toarrow [
       tfmap (ttuple [ty1; tleakable ty2])
     ; tfmap (ttuple [ty1; tleakable ty2])
     ; tdistr ty2
   ] tbool)
-let f_undeclassify_invariant_fmap ty1 ty2 f1 f2 f3 =
+let f_secrndasgn_invariant_fmap ty1 ty2 f1 f2 f3 =
 (*   Printf.printf "f1 type: %s\n" (dump_ty f1.f_ty); *)
 (*   Printf.printf "f2 type: %s\n" (dump_ty f2.f_ty); *)
 (*   let ty1 = proj_fmap_ty 0 env f1.f_ty in *)
 (*   Printf.printf "t1: %s\n" (dump_ty ty1); *)
 (*   let ty2 = proj_fmap_ty 1 env f1.f_ty in *)
 (*   Printf.printf "t2: %s\n" (dump_ty ty2); *)
-(*   f_app (fop_undeclassify_invariant_fmap ty1 ty2) [f1; f2] tbool *)
-  f_app (fop_undeclassify_invariant_fmap ty1 ty2) [f1; f2; f3] tbool
+(*   f_app (fop_secrndasgn_invariant_fmap ty1 ty2) [f1; f2] tbool *)
+  f_app (fop_secrndasgn_invariant_fmap ty1 ty2) [f1; f2; f3] tbool
 (* -------------------------------------------------------------------- *)
 let f_losslessF f = f_bdHoareF f_true f f_true FHeq f_r1
 
