src/ecFol.mli
@@ -77,7 +77,7 @@ val f_inst         : EcTypes.ty -> form -> form
 val f_secret       : form
 val f_leaked       : form
 
-val f_undeclassify_invariant_fmap : EcTypes.ty -> EcTypes.ty -> form -> form -> form -> form
+val f_secrndasgn_invariant_fmap : EcTypes.ty -> EcTypes.ty -> form -> form -> form -> form
 
 (* common functions *)
 val f_identity : ?name:EcSymbols.symbol -> EcTypes.ty -> form
