src/phl/ecPhlLeakable.mli
@@ -13,5 +13,5 @@ open EcCoreGoal.FApi
 
 (* -------------------------------------------------------------------- *)
 val process_declassify : side -> backward
-val process_secsample  : side -> backward
-val process_undeclassify : backward
+val process_secrnd  : side -> backward
+val process_secrndasgn : backward
